Paolo's proposed model adaptation.

theories/lang/cpp/model/simple_pred.v
@@ -694,7 +694,7 @@ Module SimpleCPP.
       require an extra side-condition that the code is loaded.
      *)
     Definition code_own (p : ptr) (f : Func + Method + Ctor + Dtor) : mpred :=
-      valid_ptr p **
+      strict_valid_ptr p **
       own _ghost.(code_name)
         (A := gmapUR ptr (agreeR (leibnizO (Func + Method + Ctor + Dtor))))
         {[ p := to_agree f ]}.
@@ -705,7 +705,10 @@ Module SimpleCPP.
     Lemma code_own_valid f p : code_own p f ⊢ valid_ptr p.
     Proof. iIntros "[$ _]". Qed.
     Lemma code_own_strict_valid f p : code_own p f ⊢ strict_valid_ptr p.
-    Proof. Admitted. (** TODO: this requires that we strengthen our model *)
+    Proof. iIntros "[$ _]". Qed.
+
+    Lemma code_own_valid f p : code_own p f ⊢ valid_ptr p.
+    Proof. by rewrite code_own_strict_valid strict_valid_valid. Qed.
     Definition code_at (_ : genv) (f : Func) (p : ptr) : mpred :=
       code_own p (inl (inl (inl f))).
     Definition method_at (_ : genv) (m : Method) (p : ptr) : mpred :=
